\documentclass[../rgr_2.tex]{subfiles}

\begin{document}

\Problem{Знайти розв'язок задачі Коші
$
	y''+y'-6y=0,~y(0)=1,~y'(0)=2
$
}
\Solution

\begin{align}
	\lambda^2+\lambda-6=0 \\
	\left(\lambda-2\right)\,\left(\lambda+3\right)=0 \\
	\lambda_1 = 2,
	\lambda_2 = -3 \\
	\varphi_1(x)=e^{\lambda_1 x}=e^{2x} \\
	\varphi_2(x)=e^{\lambda_2 x}=e^{-3x}
\end{align}
\begin{equation}
	W=
	\begin{vmatrix}
		e^{2x}	&e^{-3x}	\\
		2e^{2x}	&-3e^{-3x}
	\end{vmatrix}
	=-5e^{-x} \neq 0 \text{,~отже розв'язки лінійно незалежні}
\end{equation}

\begin{equation}
	y=C\,{e}^{2\,x}+\frac{C_{1}}{{e}^{3\,x}}
\end{equation}

Час знайти розв'язок задачі Коші

\begin{dmath}
	\begin{cases}
		y=C\,{e}^{2\,x}+\frac{C_{1}}{{e}^{3\,x}} \\
		y'=2\,C\,{e}^{2\,x}-\frac{3\,C_{1}}{{e}^{3\,x}}
	\end{cases}
\implies
	\begin{cases}
		1=C\,{e}^0+\frac{C_{1}}{{e}^0} \\
		2=2C-3C_1
	\end{cases}
\implies
	\begin{cases}
		1=C+C_1 \\
		2=2(1-C_1)-3C_1
	\end{cases}
\\
	\begin{cases}
		1=C+C_1 \implies C=1 \\
		0=-5C_1 \implies C_1=0
	\end{cases}
\implies y={e}^{2\,x}
\end{dmath}

\Answer{
	$
	y={e}^{2\,x}
	$
}

\end{document}
